# Indefinite Integrals of $trig^4(x)$

[Index](trig_inverse_trig_int_ref.md)

$$
\begin{aligned}
    & \int \sin^4(x) \,\mathrm{d}x = \dfrac{3x}{8} - \dfrac{\sin(2x)}{4} + \dfrac{\sin(4x)}{32} + C \\
    & \int \cos^4(x) \,\mathrm{d}x = \dfrac{3x}{8} + \dfrac{\sin(2x)}{4} + \dfrac{\sin(4x)}{32} + C  \\
    & \int \tan^4(x) \,\mathrm{d}x = \dfrac{\tan^3(x)}{3} - \tan(x) + x + C \\
    & \int \cot^4(x) \,\mathrm{d}x = -\dfrac{\cot^3(x)}{3} + \cot(x) + x + C \\
    & \int \sec^4(x) \,\mathrm{d}x = \dfrac{\tan^3(x)}{3} + \tan(x)  + C \\
    & \int \csc^4(x) \,\mathrm{d}x = -\dfrac{\cot^3(x)}{3} - \cot(x)  + C
\end{aligned}
$$

## sin

$$
\begin{aligned}
    \sin^2(x) &= \dfrac{1-\cos(2x)}{2} \\
    \therefore \int \sin^4(x) \,\mathrm{d}x &= \int \left(\dfrac{1-\cos(2x)}{2}\right)^2 \,\mathrm{d}x \\
                                            &= \dfrac{1}{4} \int (1-\cos(2x))^2 \,\mathrm{d}x \\
                                            &= \dfrac{1}{4} \int (1-2\cos(2x)+\cos^2(2x)) \,\mathrm{d}x \\
                                            &= \dfrac{1}{4} \int (1-2\cos(2x)+\dfrac{1+\cos(4x)}{2}) \,\mathrm{d}x \\
                                            &= \dfrac{1}{4} \int (\dfrac{3}{2} - 2\cos(2x) + \dfrac{\cos(4x)}{2}) \,\mathrm{d}x \\
                                            &= \dfrac{1}{4} \int \dfrac{3}{2}\,\mathrm{d}x - \dfrac{1}{2}\int \cos(2x) \,\mathrm{d}x + \dfrac{1}{8} \int \cos(4x) \,\mathrm{d}x \\
                                            &= \dfrac{3}{8}x - \dfrac{1}{4}\sin(2x) + \dfrac{1}{32}\sin(4x) + C

\end{aligned}
$$

## cos

$$
\begin{aligned}
    \cos^2(x) &= \dfrac{1 + \cos(2x)}{2} \\
    \therefore \int \cos^4(x) \,\mathrm{d}x &= \int \left(\dfrac{1 + \cos(2x)}{2}\right)^2 \,\mathrm{d}x \\
                                            &= \dfrac{1}{4} \int (1 + \cos(2x))^2 \,\mathrm{d}x \\
                                            &= \dfrac{1}{4} \int (1 + 2\cos(2x) + \cos^2(2x)) \,\mathrm{d}x \\
                                            &= \dfrac{1}{4} \int (1 + 2\cos(2x) + \dfrac{1+\cos(4x)}{2}) \,\mathrm{d}x \\
                                            &= \dfrac{1}{4} \int (\dfrac{3}{2} + 2\cos(2x) + \dfrac{\cos(4x)}{2}) \,\mathrm{d}x \\
                                            &= \dfrac{1}{4} \int \dfrac{3}{2}\,\mathrm{d}x + \dfrac{1}{2}\int \cos(2x) \,\mathrm{d}x + \dfrac{1}{8} \int \cos(4x) \,\mathrm{d}x \\
                                            &= \dfrac{3}{8}x + \dfrac{1}{4}\sin(2x) + \dfrac{1}{32}\sin(4x) + C

\end{aligned}
$$

## tan

$$
\begin{aligned}
    \int \tan^2(x) \,\mathrm{d}x &= \tan(x) - x + C \\
\\
\therefore
    \int \tan^4(x) \,\mathrm{d}x &= \int \tan^2(x)\tan^2(x) \,\mathrm{d}x \\
                                 &= \int \tan^2(x)(\sec^2(x) - 1) \,\mathrm{d}x \\
                                 &= \int (\tan^2(x)\sec^2(x) - \tan^2(x)) \,\mathrm{d}x \\
                                 &= \int \tan^2(x)\sec^2(x) \,\mathrm{d}x - \int \tan^2(x) \,\mathrm{d}x \\
                                 &= \int \tan^2(x) \,\mathrm{d}\tan(x) - \int \tan^2(x) \,\mathrm{d}x \\
                                 &= \dfrac{\tan^3(x)}{3} - \tan(x) + x + C \\
\end{aligned}
$$

## cot

$$
\begin{aligned}
    \int \cot^2(x) \,\mathrm{d}x &= -\cot(x) - x + C  \\
\\
\therefore
    \int \cot^4(x) \,\mathrm{d}x &= \int \cot^2(x)\cot^2(x) \,\mathrm{d}x \\
                                 &= \int \cot^2(x)(\csc^2(x) - 1) \,\mathrm{d}x \\
                                 &= \int (\cot^2(x)\csc^2(x) - \cot^2(x)) \,\mathrm{d}x \\
                                 &= \int \cot^2(x)\csc^2(x) \,\mathrm{d}x - \int \cot^2(x) \,\mathrm{d}x \\
                                 &= -\int \cot^2(x) \,\mathrm{d}\cot(x) - \int \cot^2(x) \,\mathrm{d}x \\
                                 &= -\dfrac{\cot^3(x)}{3} + \cot(x) + x + C\\
\end{aligned}
$$

## sec

$$
\begin{aligned}
    \dfrac{\mathrm{d}}{\mathrm{d}x} \tan(x) &= \sec^2(x) \\
    \int \sec^2(x) \,\mathrm{d}x &= \tan(x) + C \\

\\
\therefore
    \int \sec^4(x) \,\mathrm{d}x &= \int \sec^2(x)\sec^2(x) \,\mathrm{d}x \\
                                 &= \int \sec^2(x)(\tan^2(x) + 1) \,\mathrm{d}x \\
                                 &= \int (\sec^2(x)\tan^2(x) + \sec^2(x)) \,\mathrm{d}x \\
                                 &= \int \sec^2(x)\tan^2(x) \,\mathrm{d}x + \int \sec^2(x) \,\mathrm{d}x \\
                                 &= \int \tan^2(x) \,\mathrm{d}\tan(x) + \int \sec^2(x) \,\mathrm{d}x \\
                                 &= \dfrac{\tan^3(x)}{3} + \tan(x)  + C
    
\end{aligned}
$$

## csc

$$
\begin{aligned}
    \dfrac{\mathrm{d}}{\mathrm{d}x} \cot(x) &= -\csc^2(x) \\
    \int \csc^2(x) \,\mathrm{d}x &= -\cot(x) + C \\

\\
\therefore
    \int \csc^4(x) \,\mathrm{d}x &= \int \csc^2(x)\csc^2(x) \,\mathrm{d}x \\
                                 &= \int \csc^2(x)(\cot^2(x) + 1) \,\mathrm{d}x \\
                                 &= \int (\csc^2(x)\cot^2(x) + \csc^2(x)) \,\mathrm{d}x \\
                                 &= \int \csc^2(x)\cot^2(x) \,\mathrm{d}x + \int \csc^2(x) \,\mathrm{d}x \\
                                 &= -\int \cot^2(x) \,\mathrm{d}\cot(x) + \int \csc^2(x) \,\mathrm{d}x \\
                                 &= -\dfrac{\cot^3(x)}{3} - \cot(x)  + C
    
\end{aligned}
$$

<script>
MathJax = {
  tex: {
    inlineMath: [['$', '$'], ['\\(', '\\)']]
  }
};
</script>
<script id="MathJax-script" async
  src="https://cdn.jsdelivr.net/npm/mathjax@3/es5/tex-chtml.js">
</script>

<script src="https://giscus.app/client.js"
        data-repo="iridiumcao/iridiumcao.github.io"
        data-repo-id="MDEwOlJlcG9zaXRvcnkyOTUwNTIyODQ="
        data-category="Announcements"
        data-category-id="DIC_kwDOEZYj_M4Cxfqj"
        data-mapping="pathname"
        data-strict="0"
        data-reactions-enabled="1"
        data-emit-metadata="0"
        data-input-position="bottom"
        data-theme="preferred_color_scheme"
        data-lang="en"
        crossorigin="anonymous"
        async>
</script>